Prove invariant for client

fairneris/examples/stenning_code.v
@@ -8,6 +8,7 @@ From fairneris.examples Require Import stenning_model.
 From fairneris.aneris_lang Require Import proofmode.
 From fairneris.aneris_lang.state_interp Require Import state_interp state_interp_events.
 From fairneris.aneris_lang.program_logic Require Import aneris_weakestpre.
+From fairneris.lib Require Import gen_heap_light.
 
 Definition client (sa_clt sa_srv : socket_address) : val :=
   λ: <>,
@@ -54,29 +55,110 @@ Canonical Structure stenning_B_stateO := leibnizO stenning_B_state.
 Class stenningG Σ := StenningG {
   stenning_A_name: gname;
   stenning_B_name: gname;
+  stenning_cnt_name: gname;
   stenning_A_G :> inG Σ (excl_authR stenning_A_stateO);
   stenning_B_G :> inG Σ (excl_authR stenning_B_stateO);
+  stenning_cnt_G :> inG Σ (authR (gen_heapUR socket_address Z));
  }.
 Class stenningPreG Σ := {
   stenning_A_PreG :> inG Σ (excl_authR stenning_A_stateO);
   stenning_B_PreG :> inG Σ (excl_authR stenning_B_stateO);
+  stenning_cnt_PreG :> inG Σ (authR (gen_heapUR socket_address Z));
  }.
 Definition stenningΣ : gFunctors :=
   #[ anerisΣ (live_model_of_user stenning_model net_model);
      GFunctor (excl_authR stenning_A_stateO);
-     GFunctor (excl_authR stenning_B_stateO) ].
+     GFunctor (excl_authR stenning_B_stateO);
+     GFunctor (authR (gen_heapUR socket_address Z))
+  ].
 
 Global Instance subG_stenningΣ {Σ} : subG stenningΣ Σ → stenningPreG Σ.
 Proof. solve_inG. Qed.
+
+Definition mAB_in (n : Z) (S: gset message) : Prop :=
+  ∃ msg, msg ∈ S ∧ good_message true n (Some msg).
+Definition mBA_in (n : Z) (S: gset message) : Prop :=
+  ∃ msg, msg ∈ S ∧ good_message false n (Some msg).
+
+Definition client_RT (n : Z) (R T : gset message) : Prop :=
+  (∀ m, mBA_in m R → mAB_in m T) ∧
+  (∀ m, m >= n → ¬ mBA_in m R)%Z.
+
+Definition server_RT (n : Z) (R T : gset message) : Prop :=
+  (∀ m, mBA_in m R → mAB_in m T) ∧
+  (∀ m, m >= n → ¬ mBA_in m R)%Z.
+
+Definition garbage_message b msg := ∀ m, ¬ good_message b m (Some msg).
+
+Lemma client_RT_good msg n R T :
+  good_message false n (Some msg) →
+  client_RT n R T →
+  client_RT (n + 1) ({[msg]} ∪ R) ({[ mAB n ]} ∪ T).
+Proof.
+  intros Hg (HRT & Hnin). split_and!.
+  - intros m [msgm [[Hin%elem_of_singleton | Hin]%elem_of_union Hgoodm]].
+    + simplify_eq.
+      have -> : n = m by eapply good_message_inj.
+      exists (mAB m). split; [set_solver|]. exists (mAB m). split_and!; try naive_solver. simpl.
+      rewrite ZOfString_inv //.
+    + have [x [??]] : mAB_in m T.
+      * apply HRT. by exists msgm.
+      * exists x. naive_solver set_solver.
+  - intros m Hm [msg' [[Hin%elem_of_singleton | Hin]%elem_of_union ?]].
+    + simplify_eq. have ? : n = m by eapply good_message_inj. lia.
+    + ospecialize (Hnin m _). lia. apply Hnin. exists msg'. naive_solver.
+Qed.
+
+Lemma client_RT_garbage n G R T :
+  (∀ msg, msg ∈ G → garbage_message false msg) →
+  client_RT n R T →
+  client_RT n (G ∪ R) ({[ mAB n ]} ∪ T).
+Proof.
+  intros Hgar (HRT & Hnin). split_and!.
+  - intros m [msgm [[Hin | Hin]%elem_of_union Hgoodm]].
+    + exfalso. eapply (Hgar msgm Hin m Hgoodm).
+    + have [x [??]] : mAB_in m T.
+      * apply HRT. by exists msgm.
+      * exists x. naive_solver set_solver.
+  - intros m Hm [msgm [[Hin | Hin]%elem_of_union Hgoodm]].
+    + exfalso. eapply (Hgar msgm Hin m Hgoodm).
+    + ospecialize (Hnin m _). lia. apply Hnin. exists msgm. naive_solver.
+Qed.
+
+Lemma client_RT_garbage_emp n R T :
+  client_RT n R T →
+  client_RT n R ({[ mAB n ]} ∪ T).
+Proof.
+  pose proof (client_RT_garbage n ∅ R T) as Hccl.
+  replace (∅ ∪ R) with R in Hccl by set_solver.
+  intros ?. apply Hccl=>//.
+Qed.
+
+Lemma client_RT_garbage_singleton n msg R T :
+  (garbage_message false msg) →
+  client_RT n R T →
+  client_RT n ({[ msg ]} ∪ R) ({[ mAB n ]} ∪ T).
+Proof.
+  intros **. eapply client_RT_garbage=>//. naive_solver set_solver.
+Qed.
 
 Section with_Σ.
   Context `{anerisG _ _ (live_model_of_user stenning_model net_model) Σ}.
   Context `{!stenningG Σ}.
   Let Ns := nroot .@ "stenning".
+  Let Nc := nroot .@ "counter".
+  Definition counter_inv :=
+    inv Nc (∃ w, gen_heap_light_ctx (L:=socket_address) (V:=Z) stenning_cnt_name w)%I.
+
+  Notation "a ↦c{ q } s" := (lmapsto (L:=socket_address) (V:=Z) stenning_cnt_name a q s)
+    (at level 20, q at level 50, format "a  ↦c{ q }  s") : bi_scope.
+
+  Notation "a ↦c s" := (lmapsto (L:=socket_address) (V:=Z) stenning_cnt_name a 1%Qp s)
+    (at level 20, format "a  ↦c  s") : bi_scope.
 
   Definition retinv : iProp Σ := frag_free_roles_are ∅ ∗
      ∃ stA stB, frag_model_is (stA, stB) ∗ own stenning_A_name (●E stA) ∗ own stenning_B_name (●E stB) ∗
-      ⌜ let (n, m) := stenning_get_n (stA, stB) in (n = m ∨ n + 1 = m)%Z ⌝.
+      let (n, m) := stenning_get_n (stA, stB) in ⌜ (n = m ∨ n = m + 1)%Z ⌝ ∗ saA ↦c{1/4} n ∗ saB ↦c{1/4} m.
 
   Lemma token_update γ {A: ofe} {_: inG Σ (excl_authR A)} (st st' st'' : A) :
     own γ (●E st) ∗ own γ (◯E st'') ==∗ own γ (●E st') ∗ own γ (◯E st').
@@ -95,15 +177,26 @@ Section with_Σ.
   Definition ipA := ip_of_address saA.
   Definition ipB := ip_of_address saB.
 
+  Definition client_si (m : message) : iProp Σ :=
+    ∃ (n : Z), ⌜ m_body m = StringOfZ n ⌝ ∗
+         saA ↦c{1/4} n ∗
+         saB ↦c{1/4} n
+  .
+
+  Definition server_si (m : message) : iProp Σ :=
+    ∃ (n : Z), ⌜ m_body m = StringOfZ n ⌝ ∗
+         saA ↦c{1/4} n ∗
+         saB ↦c{1/4} (n - 1)%Z.
+
   Lemma wp_client tid (f : nat) (Hf: f > 40) :
-    {{{ inv Ns retinv ∗ is_node ipA ∗ saA ⤇ (λ msg, ⌜ msg = msg⌝) ∗ saB ⤇ (λ msg, ⌜ msg = msg⌝) ∗
-          own stenning_A_name (◯E (ASending 0)) ∗
+    {{{ inv Ns retinv ∗ counter_inv ∗ is_node ipA ∗ saA ⤇ client_si ∗ saB ⤇ server_si ∗
+          own stenning_A_name (◯E (ASending 0)) ∗ saA ↦c{1/2} 0%Z ∗ saA ↦c{1/4} 0%Z ∗ saB ↦c{1/4} (-1)%Z ∗
           (ipA, tid) ↦M {[ Arole := f ]} ∗ saA ⤳ (∅, ∅) ∗
           free_ports (ip_of_address saA) {[port_of_address saA]} }}}
       (mkExpr (ip_of_address saA) (client saA saB #())) @ (ipA, tid); ⊤
     {{{ v, RET v; (ipA, tid) ↦M ∅ }}}.
   Proof.
-    iIntros (Φ) "(#Hinv&#Hin&#HsA&#HsB&Hst&Hf&HRT&Hfp) HΦ".
+    iIntros (Φ) "(#Hinv&#Hcinv&#Hin&#HsA&#HsB&Hst&Hcc&Hccm&Hcs&Hf&HRT&Hfp) HΦ".
     rewrite /client.
     wp_pure _.
 
@@ -133,14 +226,23 @@ Section with_Σ.
     { iExists _. iFrame. iPureIntro. lia. }
     clear f Hf.
 
-    iAssert (∃ R T, saA ⤳ (R, T))%I with "[HRT]" as (R T) "HRT".
-    { iExists _, _. iFrame. }
+    remember (0%Z) as n eqn:Heq.
+    replace 0%Z with n by naive_solver.
+    replace (ASending 0) with (ASending n) by naive_solver.
+    replace (-1)%Z with (n-1)%Z by naive_solver.
 
-    remember 0 as n eqn:Heq.
-    replace (ASending 0) with (ASending n); last naive_solver.
+    iDestruct "Hcc" as "[Hcc Hcc']".
+    iAssert (∃ R T, saA ⤳ (R, T) ∗ ⌜ client_RT n R T ⌝ ∗ (⌜ mAB n ∉ T ⌝ -∗ saA ↦c{1/4} n ∗ saB ↦c{1/4} (n-1)%Z))%I
+      with "[HRT Hccm Hcs]" as (R T) "(HRT & HinvRT & Hccm)".
+    { iExists _, _. iFrame. iSplit; last naive_solver. rewrite /client_RT. iPureIntro.
+      split_and!; try naive_solver set_solver. }
 
-    assert (n >= 0) as Hn; first lia. clear Heq.
+    iCombine "Hcc Hcc'" as "Hcc".
+
+    assert (n >= 0)%Z as Hn; first lia. clear Heq.
     iLöb as "IH" forall (f' n Hn R T) "Hf". iDestruct "Hf'" as %Hf.
+
+    iDestruct "HinvRT" as %HinvRT.
 
     wp_pure _.
     wp_pure _.
@@ -149,7 +251,10 @@ Section with_Σ.
     iApply sswp_MU_wp_fupd.
 
     iInv Ns as "Hi" "Hclose". iModIntro.
-    iApply (wp_send _ _ false with "[Hsh] [HRT] [HsA]")=>//=>//=>//.
+    iApply (wp_send _ _ (if decide (mAB n ∈ T) then true else false) with "[Hsh] [HRT] [] [HsA Hccm]")=>//=>//=>//.
+    { destruct (decide _); first naive_solver.
+      iSpecialize ("Hccm" with "[//]"). rewrite /server_si //. iNext. iExists n. iSplit=>//.  }
+
     iNext. iIntros "Hsh HRT".
     iDestruct "Hi" as "(Hfr & %stA & %stB & Hmod & HstA & HstB)".
     iDestruct (token_agree with "HstA Hst") as %->.
@@ -168,10 +273,13 @@ Section with_Σ.
 
     wp_bind (ReceiveFrom _).
     iApply sswp_MU_wp_fupd.
-    iInv Ns as "Hi" "Hclose". iModIntro.
+    iInv Ns as "Hi" "Hclose". iInv Nc as "Hw" "Hclose'". iModIntro.
 
     iApply (wp_recv with "[Hsh] [HRT] [HsB]")=>//=>//=>//.
-    iNext. clear stB. iDestruct "Hi" as "(Hfr & %stA & %stB & Hmod & HstA & HstB & %Hnm)".
+    iNext. clear stB. iDestruct "Hi" as "(Hfr & %stA & %stB & Hmod & HstA & HstB & Hcounters)".
+    rewrite /stenning_get_n /=. iDestruct "Hcounters" as "(%Hcrel & Hcci & Hcsi)".
+    iDestruct "Hw" as (w) "Hw".
+
     iDestruct (token_agree with "HstA Hst") as %->.
 
     iIntros (om r) "Hmsg".
@@ -182,26 +290,51 @@ Section with_Σ.
     destruct (decide (good_message false n omsg)) as [[msg Hgood]|Hbad].
     - iDestruct "Hmsg" as "[(-> & %Heq & Hsh & HRT)|(%msg' & -> & %Heq & %Heqdest & Hsh & HRT & Hnew)]".
       { simplify_eq. naive_solver. }
-      destruct Hgood as (?&Hbody&?&?). simplify_eq.
+
+      iAssert (⌜ msg ∉ R ⌝)%I as %HnR.
+      { iPureIntro. destruct HinvRT as (?&Hnin). intros Hc. apply (Hnin n). lia.
+        exists msg. split=>//. simplify_eq. eexists. naive_solver. }
+      simplify_eq.
+
+      iSpecialize ("Hnew" with "[]").
+      { naive_solver. }
+      iDestruct "Hnew" as (j) "(%Hbody' & Hcc' & Hcs)".
+      iDestruct (lmapsto_agree with "Hcc' Hcc") as %->.
+      iDestruct (lmapsto_agree with "Hcs Hcsi") as %Hcseq.
+
+      iCombine "Hcc Hcci Hcc'" as "Hcc".
+      replace (1/2 + (1/4 + 1/4))%Qp with 1%Qp; last first.
+      { admit. (* Q reasonning *) }
+      iDestruct (gen_heap_light_update (L:=socket_address) _ _ _ _ (n+1)%Z
+             with "Hw Hcc") as ">[Hw [Hcc [Hccm Hcci]]]".
+
+      destruct Hgood as (?&Hbody&?&?).
       iApply (mu_step_model _ _ _ _ ∅ ∅ _ ((ASending (1+n), stB) : stenning_model) with "Hmod [Hf] [Hfr //]").
-      { constructor. exists msg'. naive_solver. }
+      { constructor. exists msg. naive_solver. }
       { set_solver. }
       { set_solver. }
       { rewrite fmap_empty map_union_empty. done. }
       iIntros "Hmod Hf Hfr".
       rewrite map_union_empty /usr_fl /=.
       iMod (token_update with "[$HstA $Hst]") as "[HstA Hst]".
-      iMod ("Hclose" with "[Hfr Hmod HstA HstB]").
-      { iNext. rewrite /retinv. iFrame. iExists (ASending (1+n)), _. iFrame. admit. }
+      iMod ("Hclose'" with "[Hw]"); first naive_solver.
+      iMod ("Hclose" with "[Hfr Hmod HstA HstB Hcci Hcsi]").
+      { iNext. rewrite /retinv. iFrame. iExists (ASending (1+n)), _. iFrame.
+        rewrite /stenning_get_n /= -Hcseq. iSplit.
+        * iPureIntro. right. lia.
+        * rewrite Z.add_comm. admit. (* Qp reasonning. *) }
       iModIntro. iApply wp_value'. do 5 wp_pure _.
-      rewrite bool_decide_true; last by do 2 f_equal.
+      clear Hcseq.
+      simplify_eq. rewrite bool_decide_true; last by do 2 f_equal.
       do 3 wp_pure _.
       { simpl. rewrite Hbody //. }
       do 4 wp_pure _. rewrite bool_decide_true //. do 2 wp_pure _.
-      iApply ("IH" with "[] [Hst] [$] [$] [] [$HRT] [$]").
+      iApply ("IH" with "[] [Hst] [$] [$Hsh] [] [$HRT] [] [Hccm Hcs] [$Hcc] [$Hf]").
       { iPureIntro; lia. }
       { rewrite Z.add_comm //. }
       { iPureIntro; lia. }
+      { iPureIntro. apply client_RT_good=>//. exists msg. naive_solver. }
+      { iIntros. replace (n + 1 - 1)%Z with n by lia. iFrame. admit. (* Qp *) }
     - iApply (mu_step_model _ _ _ _ ∅ ∅ _ ((ASending n, stB) : stenning_model) with "Hmod [Hf] [Hfr //]").
       { simpl. by apply A_RecvFail. }
       { set_solver. }
@@ -209,23 +342,53 @@ Section with_Σ.
       { rewrite fmap_empty map_union_empty. done. }
       iIntros "Hmod Hf Hfr".
       rewrite map_union_empty /usr_fl /=.
+
       iMod (token_update with "[$HstA $Hst]") as "[HstA Hst]".
-      iMod ("Hclose" with "[Hfr Hmod HstA HstB]").
-      { iNext. rewrite /retinv. iFrame. iExists (ASending n), _. iFrame. admit. }
+      iMod ("Hclose'" with "[Hw]"); first naive_solver.
+      iMod ("Hclose" with "[Hfr Hmod HstA HstB Hcci Hcsi]").
+      { iNext. rewrite /retinv. iFrame. iExists (ASending n), _. iFrame. simpl. iPureIntro. naive_solver. }
       iModIntro. iApply wp_value'. simpl.
       iDestruct "Hmsg" as "[(-> & %Heq & Hsh & HRT)|(%msg & -> & %Heq & %Heqdest & Hsh & HRT & Hnew)]".
-      + do 3 wp_pure _. iApply ("IH" with "[] [Hst] [$] [$] [] [$HRT] [$]")=>//.
+      + do 3 wp_pure _. iApply ("IH" with "[] [$Hst] [$] [$Hsh] [] [$HRT] [] [] [$Hcc] [$Hf]").
+        { iPureIntro; lia. }
+        { iPureIntro; lia. }
+        { iPureIntro. by apply client_RT_garbage_emp. }
+        { iIntros (Hnin). exfalso. apply Hnin. set_solver. }
       + do 5 wp_pure _. destruct (decide (m_sender msg = saB)); last first.
         { rewrite bool_decide_false; last naive_solver. wp_pure _.
-          iApply ("IH" with "[] [Hst] [$] [$] [] [$HRT] [$]")=>//. }
+          iApply ("IH" with "[] [$Hst] [$] [$Hsh] [] [$HRT] [] [] [$Hcc] [$Hf]").
+          { iPureIntro; lia. }
+          { iPureIntro; lia. }
+          { iPureIntro. apply client_RT_garbage_singleton=>//.
+            intros m. rewrite /good_message. naive_solver. }
+          { iIntros (Hnin). exfalso. apply Hnin. set_solver. } }
         rewrite bool_decide_true //; last by do 2 f_equal. do 2 wp_pure _.
         destruct (ZOfString (m_body msg)) as [msg_n|] eqn:Heqmsg; last first.
         { wp_pure _. rewrite /= Heqmsg //. do 5 wp_pure _.
-          iApply ("IH" with "[] [Hst] [$] [$] [] [$HRT] [$]")=>//. }
+          iApply ("IH" with "[] [$Hst] [$] [$Hsh] [] [$HRT] [] [] [$Hcc] [$Hf]").
+          { iPureIntro; lia. }
+          { iPureIntro; lia. }
+          { iPureIntro. apply client_RT_garbage_singleton=>//.
+            intros m. rewrite /good_message. naive_solver. }
+          { iIntros (Hnin). exfalso. apply Hnin. set_solver. } }
         wp_pure _. rewrite /= Heqmsg //. do 4 wp_pure _.
-        rewrite bool_decide_false; last first.
+        have Hwrongn : msg_n ≠ n.
         { intros Hc. simplify_eq. apply Hbad. eexists; split=>//. }
-        wp_pure _. iApply ("IH" with "[] [Hst] [$] [$] [] [$HRT] [$]")=>//.
+        rewrite bool_decide_false //; last naive_solver. wp_pure _.
+
+        iAssert (⌜ msg ∈ R ⌝)%I with "[Hnew Hcc]" as %Hin.
+        { destruct (decide (msg ∈ R)) as [|Hnin]=>//. iSpecialize ("Hnew" $! Hnin).
+          rewrite /client_si.
+          iDestruct "Hnew" as (n') "(%Hbody & Hcc' & _)".
+          iDestruct (lmapsto_agree with "Hcc' Hcc") as %->.
+          rewrite Hbody ZOfString_inv in Heqmsg. simplify_eq. }
+
+        iApply ("IH" with "[] [$Hst] [$] [$Hsh] [] [$HRT] [] [] [$Hcc] [$Hf]").
+        { iPureIntro; lia. }
+        { iPureIntro; lia. }
+        { iPureIntro. replace ({[msg]} ∪ R) with R by set_solver.
+          apply client_RT_garbage_emp=>//. }
+        { iIntros (Hnin). exfalso. apply Hnin. set_solver. }
   Admitted.
 
   Lemma wp_server tid (f : nat) (Hf: f > 40) :
